Rewrite.

theories/std/option.v
@@ -11,35 +11,35 @@ From zoo Require Import
 Implicit Types v : val.
 
 Notation "'None'" := (
-  in_type "opt" 0
+  in_type "option" 0
 )(in custom zoo_tag
 ).
 Notation "'Some'" := (
-  in_type "opt" 1
+  in_type "option" 1
 )(in custom zoo_tag
 ).
 
-Coercion opt_to_val o :=
+Coercion option_to_val o :=
   match o with
   | None =>
       §None
   | Some v =>
       ’Some{ v }
   end.
-#[global] Arguments opt_to_val !_ / : assert.
+#[global] Arguments option_to_val !_ / : assert.
 
-#[global] Instance opt_to_val_inj' :
-  Inj (=) val_eq opt_to_val.
+#[global] Instance option_to_val_inj' :
+  Inj (=) val_eq option_to_val.
 Proof.
   intros [] []; naive_solver.
 Qed.
-#[global] Instance opt_to_val_inj :
-  Inj (=) (=) opt_to_val.
+#[global] Instance option_to_val_inj :
+  Inj (=) (=) option_to_val.
 Proof.
   intros ?* ->%eq_val_eq%(inj _). done.
 Qed.
-#[global] Instance opt_to_val_physical o :
-  ValPhysical (opt_to_val o).
+#[global] Instance option_to_val_physical o :
+  ValPhysical (option_to_val o).
 Proof.
   destruct o; done.
 Qed.
@@ -48,17 +48,17 @@ Section zoo_G.
   Context `{zoo_G : !ZooG Σ}.
   Context τ `{!iType (iPropI Σ) τ}.
 
-  Definition itype_opt t : iProp Σ :=
+  Definition itype_option t : iProp Σ :=
       ⌜t = §None⌝
     ∨ ∃ v, ⌜t = ’Some{ v }⌝ ∗ τ v.
-  #[global] Instance itype_opt_itype :
-    iType _ itype_opt.
+  #[global] Instance itype_option_itype :
+    iType _ itype_option.
   Proof.
     split. apply _.
   Qed.
 
-  Lemma wp_match_opt t e1 x e2 Φ :
-    itype_opt t -∗
+  Lemma wp_match_option t e1 x e2 Φ :
+    itype_option t -∗
     ( WP e1 {{ Φ }} ∧
       ∀ v, τ v -∗ WP subst' x v e2 {{ Φ }}
     ) -∗
