theories/saturn/mpmc_stack_1.v
@@ -10,7 +10,7 @@ From zoo.language Require Import
   notations
   diaframe.
 From zoo.std Require Import
-  opt
+  option
   lst.
 From zoo.saturn Require Export
   base.
