theories/saturn/mpsc_queue_3.v
@@ -13,7 +13,7 @@ From zoo.language Require Import
   notations
   diaframe.
 From zoo.std Require Import
-  opt
+  option
   clst.
 From zoo.saturn Require Export
   base.
