theories/saturn/spsc_bqueue.v
@@ -19,7 +19,7 @@ From zoo.language Require Import
   notations
   diaframe.
 From zoo.std Require Import
-  opt
+  option
   array.
 From zoo.saturn Require Export
   base.
