theories/std/dynarray_2.v
@@ -18,7 +18,7 @@ From zoo.std Require Import
   assume
   math
   ref_
-  opt
+  option
   array.
 From zoo Require Import
   options.
@@ -657,7 +657,7 @@ Section zoo_G.
   Context τ `{!iType (iPropI Σ) τ}.
 
   #[local] Definition itype_slot :=
-    itype_opt (itype_ref τ).
+    itype_option (itype_ref τ).
   Definition itype_dynarray t : iProp Σ :=
     ∃ l,
     ⌜t = #l⌝ ∗
@@ -795,7 +795,7 @@ Section zoo_G.
     wp_rec.
     wp_smart_apply (dynarray_data_type with "Htype") as "%cap %data #Hdata_type".
     wp_apply (array_get_type with "Hdata_type") as "%slot (%Hi & #Hslot)".
-    wp_apply (wp_match_opt with "Hslot"). iSplit.
+    wp_apply (wp_match_option with "Hslot"). iSplit.
     - wp_apply diverge_spec.
     - iIntros "%r #Hr /=".
       wp_apply (ref_get_type with "Hr").
@@ -817,7 +817,7 @@ Section zoo_G.
     wp_rec.
     wp_smart_apply (dynarray_data_type with "Htype") as "%cap %data #Hdata_type".
     wp_apply (array_get_type with "Hdata_type") as "%slot (%Hi & #Hslot)".
-    wp_apply (wp_match_opt with "Hslot"). iSplit.
+    wp_apply (wp_match_option with "Hslot"). iSplit.
     - wp_apply diverge_spec.
     - iIntros "%r #Hr /=".
       wp_apply (ref_set_type with "[$Hr $Hv]").
@@ -941,7 +941,7 @@ Section zoo_G.
     wp_smart_apply assume_spec' as "%Hcap".
     wp_smart_apply assume_spec' as "%Hsz".
     wp_smart_apply (array_unsafe_get_type with "Hdata_type") as "%slot #Hslot"; first lia.
-    wp_apply (wp_match_opt with "Hslot"). iSplit.
+    wp_apply (wp_match_option with "Hslot"). iSplit.
     - wp_apply diverge_spec.
     - iIntros "%r #Hr /=".
       wp_smart_apply (array_unsafe_set_type with "[$Hdata_type]") as "_"; [lia | iSteps |].
