theories/std/optional.v
@@ -1,0 +1,102 @@
+From zoo Require Import
+  prelude.
+From zoo.language Require Import
+  notations
+  diaframe.
+From zoo.std Require Export
+  base.
+From zoo Require Import
+  options.
+
+Implicit Types v : val.
+
+Inductive optional {A} :=
+  | Nothing
+  | Anything
+  | Something (a : A).
+#[global] Arguments optional : clear implicits.
+
+Definition option_to_optional {A} (o : option A) :=
+  match o with
+  | None =>
+      Nothing
+  | Some a =>
+      Something a
+  end.
+
+#[global] Instance Something_inj A :
+  Inj (=) (=) (@Something A).
+Proof.
+  rewrite /Inj. naive_solver.
+Qed.
+
+Notation "'Nothing'" := (
+  in_type "optional" 0
+)(in custom zoo_tag
+).
+Notation "'Anything'" := (
+  in_type "optional" 1
+)(in custom zoo_tag
+).
+Notation "'Something'" := (
+  in_type "optional" 2
+)(in custom zoo_tag
+).
+
+Coercion optional_to_val o :=
+  match o with
+  | Nothing =>
+      §Nothing
+  | Anything =>
+      §Anything
+  | Something v =>
+      ’Something{ v }
+  end.
+#[global] Arguments optional_to_val !_ / : assert.
+
+#[global] Instance optional_to_val_inj' :
+  Inj (=) val_eq optional_to_val.
+Proof.
+  intros [] []; naive_solver.
+Qed.
+#[global] Instance optional_to_val_inj :
+  Inj (=) (=) optional_to_val.
+Proof.
+  intros ?* ->%eq_val_eq%(inj _). done.
+Qed.
+#[global] Instance optional_to_val_physical o :
+  ValPhysical (optional_to_val o).
+Proof.
+  destruct o; done.
+Qed.
+
+Section zoo_G.
+  Context `{zoo_G : !ZooG Σ}.
+  Context τ `{!iType (iPropI Σ) τ}.
+
+  Definition itype_optional t : iProp Σ :=
+      ⌜t = §Nothing⌝
+    ∨ ⌜t = §Anything⌝
+    ∨ ∃ v, ⌜t = ’Something{ v }⌝ ∗ τ v.
+  #[global] Instance itype_optional_itype :
+    iType _ itype_optional.
+  Proof.
+    split. apply _.
+  Qed.
+
+  Lemma wp_match_optional t e1 e2 x e3 Φ :
+    itype_optional t -∗
+    ( WP e1 {{ Φ }} ∧
+      WP e2 {{ Φ }} ∧
+      ∀ v, τ v -∗ WP subst' x v e3 {{ Φ }}
+    ) -∗
+    WP match: t with Nothing => e1 | Anything => e2 | Something x => e3 end {{ Φ }}.
+  Proof.
+    iIntros "[-> | [-> | (%v & -> & #Hv)]] H".
+    1: rewrite bi.and_elim_l.
+    2,3: rewrite bi.and_elim_r.
+    2: rewrite bi.and_elim_l.
+    3: rewrite bi.and_elim_r.
+    all: iSteps.
+  Qed.
+End zoo_G.
